Regular language equivalency

Regex/Algorithm/Defs.lean
@@ -1,67 +1,67 @@
 import Regex.Parse
 
 namespace Regex
-variable {α : Type u} [deq : DecidableEq α] {r : Regex α}
+variable {α : Type u} [deq : DecidableEq α] {r : Regex α} {w : List α}
 
 /-- Various actions the match stack can execute -/
-inductive Action (α : Type u) : Type u where
+inductive Action (w : List α) : Type u where
   /-- Start a regex match (and maybe finish it). -/
-  | regex (r : Regex α) (w : List α) (s : ℕ) (cap : Captures) : Action α
+  | regex (r : Regex α) (s : Pos w) (cap : Captures w) : Action w
   /-- Wait for matches from the first regex of a concatenation -/
-  | concatWait (r : Regex α) (w : List α) : Action α
+  | concatWait (r : Regex α) : Action w
   /-- Process the second regex with another match -/
-  | concat (r : Regex α) (w : List α) (old new : PartialMatches) : Action α
+  | concat (r : Regex α) (old new : PartialMatches w) : Action w
   /-- Wait for matches from the first regex of an alternation -/
-  | orWait (r : Regex α) (w : List α) (s : ℕ) (cap : Captures) : Action α
+  | orWait (r : Regex α) (s : Pos w) (cap : Captures w) : Action w
   /-- Concatenate the two lists of matches -/
-  | or (fst : PartialMatches) : Action α
+  | or (fst : PartialMatches w) : Action w
   /-- Wait for matches from the first match attempt of a star -/
-  | starWait (t : StarType) (r : Regex α) (w : List α) (s : ℕ) (cap : Captures): Action α
+  | starWait (t : StarType) (r : Regex α) (s : Pos w) (cap : Captures w): Action w
   /-- Process the star with another match. This looks like `concat`,
   but has special behavior that it's not worth complicating `concat` for. -/
-  | star (t : StarType) (r : Regex α) (w : List α) (s : ℕ) (cap : Captures)
-    (old new : PartialMatches) : Action α
+  | star (t : StarType) (r : Regex α) (s : Pos w)
+    (cap : Captures w) (old new : PartialMatches w) : Action w
   /-- Capture a match -/
-  | capture (n : ℕ) (s : ℕ) : Action α
+  | capture (n : ℕ) (s : Pos w) : Action w
   deriving Repr
 
 /-- A stack of actions, along with an argument -/
 @[ext]
-structure MatchStack (α : Type*) where
-  entries : List (Action α)
-  arg : PartialMatches
+structure MatchStack (w : List α) where
+  entries : List (Action w)
+  arg : PartialMatches w
   deriving Repr
 
-def Action.process (ac : Action α) (arg : PartialMatches)
-    : MatchStack α := match ac with
-  | Action.regex r w s cap => match r with
+def Action.process (ac : Action w) (arg : PartialMatches w)
+    : MatchStack w := match ac with
+  | Action.regex r s cap => match r with
     | .bot => ⟨[], []⟩
     | .empty => ⟨[], [(s, cap)]⟩
-    | .unit c => ⟨[], if h : w[s]? = c then [(s + 1, cap)] else []⟩
-    | .concat q r => ⟨[regex q w s cap, concatWait r w], []⟩
-    | .or q r => ⟨[regex q w s cap, orWait r w s cap], []⟩
-    | .star t r => ⟨[regex r w s cap, starWait t r w s cap], []⟩
+    | .unit c => ⟨[], if h : w[s.val]? = c then [(s.succOfIndex h, cap)] else []⟩
+    | .concat q r => ⟨[regex q s cap, concatWait r], []⟩
+    | .or q r => ⟨[regex q s cap, orWait r s cap], []⟩
+    | .star t r => ⟨[regex r s cap, starWait t r s cap], []⟩
     | .start => ⟨[], if s = 0 then [(s, cap)] else []⟩
     | .end' => ⟨[], if s = w.length then [(s, cap)] else []⟩
-    | .capture n r => ⟨[regex r w s cap, capture n s], []⟩
+    | .capture n r => ⟨[regex r s cap, capture n s], []⟩
     | .backref d n => ⟨[regex (match (cap n).head? with
       | none => match d with | .bot => [/⊥/] | .empty => [//]
       | some (cs, ct) => list (w.extract cs ct)
-      ) w s cap], []⟩
-  | .concatWait r w => ⟨[concat r w arg []], []⟩
-  | .concat r w old new => match old with
+      ) s cap], []⟩
+  | .concatWait r => ⟨[concat r arg []], []⟩
+  | .concat r old new => match old with
     | [] => ⟨[], new ++ arg⟩
-    | (s', cap) :: old => ⟨[regex r w s' cap, concat r w old (new ++ arg)], []⟩
-  | .orWait r w s cap => ⟨[regex r w s cap, or arg], []⟩
+    | (s', cap) :: old => ⟨[regex r s' cap, concat r old (new ++ arg)], []⟩
+  | .orWait r s cap => ⟨[regex r s cap, or arg], []⟩
   | .or fst => ⟨[], fst ++ arg⟩
-  | .starWait t r w s cap => ⟨[star t r w s cap arg []], []⟩
-  | .star t r w s cap old new => match old with
+  | .starWait t r s cap => ⟨[star t r s cap arg []], []⟩
+  | .star t r s cap old new => match old with
     | [] => ⟨[], match t with
         | .greedy => new ++ arg ++ [(s, cap)]
         | .lazy => [(s, cap)] ++ new ++ arg⟩
-    | (s', cap) :: old => ⟨if s < s'
-        then [regex [/⟨r⟩*‹t›/] w s' cap, star t r w s cap old (new ++ arg)]
-        else [star t r w s cap old (new ++ arg ++ [(s', cap)])], []⟩
+    | (s', cap') :: old => ⟨if s < s'
+        then [regex [/⟨r⟩*‹t›/] s' cap', star t r s cap old (new ++ arg)]
+        else [star t r s cap old (new ++ arg ++ [(s', cap')])], []⟩
   | .capture n s => ⟨[], arg.map fun (s', cap) ↦
       (s', cap.update n [(s, s')])⟩
 
@@ -81,25 +81,25 @@ def Action.process (ac : Action α) (arg : PartialMatches)
 
 /-- The result of stepping the match stack. Either the next state or the
 match result -/
-def StepResult := Except PartialMatches
+def StepResult (w : List α) := Except (PartialMatches w)
   deriving Monad, LawfulMonad
 
 /-- Constructs a match stack out of a single action -/
-def Action.matchStack (ac : Action α) (arg : PartialMatches)
-    : MatchStack α := MatchStack.mk [ac] arg
+def Action.matchStack (ac : Action w) (arg : PartialMatches w)
+    : MatchStack w := MatchStack.mk [ac] arg
 
 namespace MatchStack
 
 /-- Advancing the state of the regex matches. The state steps successfully
 unless the stack is empty, in which case the list of matches is returned -/
-def step (st : MatchStack α) : StepResult (MatchStack α)
+def step (st : MatchStack w) : StepResult w (MatchStack w)
   := match st.entries with
   | [] => Except.error st.arg
   | action :: stack => let ⟨entries, return'⟩ := action.process st.arg
     Except.ok ⟨entries ++ stack, return'⟩
 
-theorem step_eq_ok {st st' : MatchStack α} (hst : st.step = Except.ok st')
-    : ∃ (ac : Action α) (as : List (Action α)), st.entries = ac :: as ∧ st' = MatchStack.mk
+theorem step_eq_ok {st st' : MatchStack w} (hst : st.step = Except.ok st')
+    : ∃ (ac : Action w) (as : List (Action w)), st.entries = ac :: as ∧ st' = MatchStack.mk
         (entries := (ac.process st.arg).entries ++ as)
         (arg := (ac.process st.arg).arg)
         := by
@@ -109,19 +109,19 @@ theorem step_eq_ok {st st' : MatchStack α} (hst : st.step = Except.ok st')
   rw [Except.ok.injEq] at hst
   exact ⟨ac, as', has, Eq.symm hst⟩
 
-theorem step_eq_error {st : MatchStack α} {mat : PartialMatches}
+theorem step_eq_error {st : MatchStack w} {mat : PartialMatches w}
     (hst : st.step = Except.error mat)
     : st.entries = [] := by
   rw [step] at hst; split at hst <;> first | assumption | simp at hst
 
-theorem step_eq_error_iff {st : MatchStack α}
+theorem step_eq_error_iff {st : MatchStack w}
     : st.step = Except.error st.arg ↔ st.entries = [] := by
   constructor
   · exact fun hst ↦ st.step_eq_error hst
   · intro hst
     rw [step, hst]
 
-theorem step_singleton (ac : Action α) (arg : PartialMatches)
+theorem step_singleton (ac : Action w) (arg : PartialMatches w)
     : (MatchStack.mk [ac] arg).step = Except.ok (ac.process arg) := by
   simp [step]
 
