Regex/Basic.lean
@@ -9,16 +9,16 @@ import Regex.List
 
 namespace Regex
 
-def decreasingStrongRec {n : ℕ} {motive : (m : ℕ) → m ≤ n → Sort u}
-    (ind : ∀ m, (mn : m ≤ n) →
-      (∀ k, (kn : k ≤ n) → (km : k > m) → motive k kn) →
-      motive m mn)
-    (m : ℕ) (mn : m ≤ n)
-    : motive m mn :=
-  ind m mn fun k kn _ ↦ decreasingStrongRec ind k kn
+--def decreasingStrongRec {n : ℕ} {motive : (m : ℕ) → m ≤ n → Sort u}
+--    (ind : ∀ m, (mn : m ≤ n) →
+--      (∀ k, (kn : k ≤ n) → (km : k > m) → motive k kn) →
+--      motive m mn)
+--    (m : ℕ) (mn : m ≤ n)
+--    : motive m mn :=
+--  ind m mn fun k kn _ ↦ decreasingStrongRec ind k kn
 
-variable {α : Type u} [deq : DecidableEq α] {r : Regex α} {w : List α}
-  {s : ℕ} {hs : s ≤ w.length} {cap : Captures}
+variable {ℓ : ℕ} {α : Type*} [deq : DecidableEq α] {r : Regex α} {w : List α}
+  {s : Pos w} {cap : Captures w}
 
 theorem StarType.map_match {α β : Type*} (f : α → β) (t : StarType) (g l : α)
     : f (match t with | .greedy => g | .lazy => l) =
@@ -30,17 +30,15 @@ theorem StarType.flatten_match {α : Type*} (t : StarType) (gg gl lg ll : α)
         | .lazy => match t with | .greedy => lg | .lazy => ll) =
       (match t with | .greedy => gg | .lazy => ll) := by rcases t <;> simp
 
-set_option linter.unusedVariables false in
-/-- Initialize a partial match stack. `s` must be in bounds. -/
-def initMatchPartial (r : Regex α) (w : List α) {s : ℕ} (hs : s ≤ w.length)
-    (cap : Captures)
-    : MatchStack α where
-  entries := [Action.regex r w s cap]
+/-- Initialize a partial match stack -/
+def initMatchPartial (r : Regex α) (w : List α) (s : Pos w) (cap : Captures w)
+    : MatchStack w where
+  entries := [Action.regex r s cap]
   arg := []
 
 /-- Whether a particular regex match terminates -/
-def Terminates (r : Regex α) (w : List α) {s : ℕ} (hs : s ≤ w.length) (cap : Captures) :=
-  (r.initMatchPartial w hs cap).Terminates
+def Terminates (r : Regex α) (w : List α) (s : Pos w) (cap : Captures w) :=
+  (r.initMatchPartial w s cap).Terminates
 
 /-! Some tactics for proving termination -/
 
@@ -187,16 +185,16 @@ end Tactic
 section MatchPartial
 open MatchStack
 
-def matchPartial (r : Regex α) (w : List α) {s : ℕ} (hs : s ≤ w.length)
-  (cap : Captures) (term : r.Terminates w hs cap)
-    : PartialMatches := (r.initMatchPartial w hs cap).run term
+def matchPartial (r : Regex α) (w : List α) (s : Pos w) (cap : Captures w)
+  (term : r.Terminates w s cap)
+    : PartialMatches w := (r.initMatchPartial w s cap).run term
 
 theorem matchPartial_terminates_iff
-    : r.Terminates w hs cap ↔ (mk [.regex r w s cap] []).Terminates := iff_of_eq rfl
+    : r.Terminates w s cap ↔ (mk [.regex r s cap] []).Terminates := iff_of_eq rfl
 
 theorem matchPartial_eq_run
-  {term : r.Terminates w hs cap}
-    : r.matchPartial w hs cap term = (mk [.regex r w s cap] []).run term := rfl
+  {term : r.Terminates w s cap}
+    : r.matchPartial w s cap term = (mk [.regex r s cap] []).run term := rfl
 
 /-- `bot` always terminates -/
 theorem terminates_bot
@@ -214,8 +212,8 @@ theorem terminates_unit {c : α}
   rw [Terminates, initMatchPartial]; step; step
 
 theorem Action.terminates_concat
-    {old new arg : PartialMatches}
-    : (MatchStack.mk [concat r w old new] arg).Terminates ↔
+    {old new arg : PartialMatches w}
+    : (MatchStack.mk [concat r old new] arg).Terminates ↔
       ∀ mat ∈ old, r.Terminates w mat.1 mat.2 := by
   constructor
   · intro term mat mem
@@ -233,8 +231,8 @@ theorem Action.terminates_concat
       use term ent List.mem_cons_self
       exact ind fun m mem ↦ term _ (List.mem_cons_of_mem _ mem)
 
-theorem Action.terminates_concatWait {r : Regex α} {arg : PartialMatches}
-    : (MatchStack.mk [concatWait r w] arg).Terminates ↔
+theorem Action.terminates_concatWait {r : Regex α} {arg : PartialMatches w}
+    : (MatchStack.mk [concatWait r] arg).Terminates ↔
       ∀ mat ∈ arg, r.Terminates w mat.1 mat.2 := by
   step only [List.append_nil]
   exact terminates_concat
@@ -261,12 +259,12 @@ theorem terminates_concat {q r : Regex α}
     rw [Action.terminates_concatWait]
     exact fun mat run ↦ term mat run
 
-theorem Action.terminates_or {fst arg : PartialMatches}
-    : (MatchStack.mk [or (α := α) fst] arg).Terminates := by step; step
+theorem Action.terminates_or {fst arg : PartialMatches w}
+    : (MatchStack.mk [or (w := w) fst] arg).Terminates := by step; step
 
 theorem Action.terminates_orWait
-    {arg : PartialMatches}
-    : (MatchStack.mk [orWait r w s cap] arg).Terminates ↔ r.Terminates w s cap := by
+    {arg : PartialMatches w}
+    : (MatchStack.mk [orWait r s cap] arg).Terminates ↔ r.Terminates w s cap := by
   constructor
   · intro term
     step at term
@@ -298,13 +296,60 @@ theorem terminates_or_comm {q r : Regex α}
     : [/⟨q⟩ | ⟨r⟩/].Terminates w s cap ↔ [/⟨r⟩ | ⟨q⟩/].Terminates w s cap := by
   simp only [terminates_or]; rw [and_comm]
 
+theorem Action.terminates_star {t : StarType}
+    {old new arg : PartialMatches w}
+    : (MatchStack.mk [star t r s cap old new] arg).Terminates ↔
+      ∀ mat ∈ old, s < mat.1 → [/⟨r⟩*‹t›/].Terminates w mat.1 mat.2 := by
+  constructor
+  · intro term mat mem slt
+    induction old generalizing cap new arg with | nil => contradiction | cons ent mat' ind =>
+      step at term
+      rw [List.mem_cons] at mem
+      split at term <;> rename_i hs
+      · run_top! at term with term' term
+        rcases mem with mem | mem
+        · exact mem ▸ term'
+        · exact ind term mem
+      · rcases mem with mem | mem
+        · exact (hs (mem ▸ slt)).elim
+        · exact ind term mem
+  · intro term
+    induction old generalizing cap new arg with | nil => step; step | cons ent mat' ind =>
+      step
+      split <;> rename_i hs
+      · run_top!
+        use term ent List.mem_cons_self hs
+        exact ind fun m mem ↦ term _ (List.mem_cons_of_mem _ mem)
+      · exact ind fun m mem ↦ term _ (List.mem_cons_of_mem _ mem)
+
+theorem Action.terminates_starWait {t : StarType} {arg : PartialMatches w}
+    : (MatchStack.mk [starWait t r s cap] arg).Terminates ↔
+      ∀ mat ∈ arg, s < mat.1 → [/⟨r⟩*‹t›/].Terminates w mat.1 mat.2 := by
+  step only [List.append_nil]
+  exact terminates_star
+
 /-- `star t r` terminates iff `r` terminates and `r` terminates for every
 advancing end position and match provided by `r` -/
 theorem terminates_star {t : StarType}
     : [/⟨r⟩*‹t›/].Terminates w s cap ↔ ∃ term : r.Terminates w s cap,
       ∀ mat ∈ r.matchPartial w s cap term,
         s < mat.1 → [/⟨r⟩*‹t›/].Terminates w mat.1 mat.2 := by
-  by_cases! s ≤ w.length
+  constructor
+  · intro term
+    rw [Terminates, initMatchPartial] at term
+    step at term
+    run_top! at term with term' term
+    use term'
+    intro mat qmat
+    rw [matchPartial] at qmat
+    rw [Action.terminates_starWait] at term
+    exact term mat qmat
+  · rintro ⟨qterm, term⟩
+    rw [Terminates, initMatchPartial] at ⊢
+    step
+    run_top! using qterm
+    rw [Action.terminates_starWait]
+    exact fun mat run ↦ term mat run
 
 /-- `start` always terminates -/
 theorem terminates_start
@@ -314,7 +359,7 @@ theorem terminates_start
 theorem terminates_end'
     : [/⊣/].Terminates w s cap := by rw [Terminates, initMatchPartial]; step; step
 
-theorem Action.terminates_capture {n : ℕ} {arg : PartialMatches}
+theorem Action.terminates_capture {n : ℕ} {arg : PartialMatches w}
     : (MatchStack.mk [capture (α := α) n s] arg).Terminates := by step; step
 
 /-- `capture emp r` terminates iff `r` terminates -/
@@ -341,12 +386,12 @@ theorem matchPartial_empty
 
 theorem matchPartial_unit {c : α}
     : matchPartial [/c/] w s cap terminates_unit
-      = if w[s]? = some c then [(s + 1, cap)] else [] := by
+      = if h : w[s.val]? = some c then [(s.succOfIndex h, cap)] else [] := by
   simp only [matchPartial_eq_run]; step; step
 
-theorem Action.concat_run {old new arg : PartialMatches}
+theorem Action.concat_run {old new arg : PartialMatches w}
     (term : ∀ mat ∈ old, r.Terminates w mat.1 mat.2)
-    : (mk [.concat r w old new] arg).run (terminates_concat.mpr term)
+    : (mk [.concat r old new] arg).run (terminates_concat.mpr term)
       = new ++ arg ++
       (old.pmap (fun ent rt ↦ r.matchPartial w ent.1 ent.2 rt) term).flatten := by
   induction old generalizing new arg with | nil => step; step | cons ent mat ind =>
@@ -359,14 +404,14 @@ theorem Action.concat_run {old new arg : PartialMatches}
       List.append_cancel_right_eq]
     rfl
 
-theorem Action.concatWait_run {r : Regex α} {arg : PartialMatches}
+theorem Action.concatWait_run {r : Regex α} {arg : PartialMatches w}
     (term : ∀ mat ∈ arg, r.Terminates w mat.1 mat.2)
-    : (mk [.concatWait r w] arg).run (terminates_concatWait.mpr term)
+    : (mk [.concatWait r] arg).run (terminates_concatWait.mpr term)
       = (arg.pmap (fun ent rt ↦ r.matchPartial w ent.1 ent.2 rt) term).flatten := by
   step only [List.append_nil]
   exact concat_run term
 
-theorem matchPartial_concat (q r : Regex α) (s : ℕ) (cap : Captures)
+theorem matchPartial_concat {q r : Regex α}
     {term : [/⟨q⟩ ⟨r⟩/].Terminates w s cap}
     : matchPartial [/⟨q⟩ ⟨r⟩/] w s cap term
       = ((q.matchPartial w s cap (terminates_concat.mp term).1).pmap
@@ -379,12 +424,12 @@ theorem matchPartial_concat (q r : Regex α) (s : ℕ) (cap : Captures)
   rw! [← matchPartial_eq_run]
   rw [Action.concatWait_run (terminates_concat.mp term).2]
 
-theorem Action.or_run {s : ℕ} {fst arg : PartialMatches}
+theorem Action.or_run {fst arg : PartialMatches w}
     : (mk [.or (α := α) fst] arg).run terminates_or = fst ++ arg := by step; step
 
-theorem Action.orWait_run {r : Regex α} {s : ℕ} {cap : Captures}
-    {arg : PartialMatches} (term : r.Terminates w s cap)
-    : (mk [.orWait r w s cap] arg).run (terminates_orWait.mpr term)
+theorem Action.orWait_run {r : Regex α} {s : Pos w} {cap : Captures w}
+    {arg : PartialMatches w} (term : r.Terminates w s cap)
+    : (mk [.orWait r s cap] arg).run (terminates_orWait.mpr term)
       = arg ++ r.matchPartial w s cap term := by step; run_top!; step; step; rfl
 
 theorem matchPartial_or {q r : Regex α}
@@ -405,40 +450,58 @@ theorem mem_matchPartial_or_comm {q r : Regex α}
       mat ∈ matchPartial [/⟨r⟩ | ⟨q⟩/] w s cap (terminates_or_comm.mp term) := by
   simp only [matchPartial_or, List.mem_append]; rw [or_comm]
 
-/-- `star t r` terminates iff `r` terminates and `r` terminates for every
-advancing end position and match provided by `r` -/
-theorem terminates_star {t : StarType}
-    : [/⟨r⟩*‹t›/].Terminates w s cap ↔ ∃ term : r.Terminates w s cap,
-      ∀ mat ∈ r.matchPartial w s cap term,
-        s < mat.1 → [/⟨r⟩*‹t›/].Terminates w mat.1 mat.2 := by
-  rw [Terminates, initMatchPartial]
+theorem Action.star_run {t : StarType} {old new arg : PartialMatches w}
+    (term : ∀ mat ∈ old, s < mat.1 → [/⟨r⟩*‹t›/].Terminates w mat.1 mat.2)
+    : (mk [.star t r s cap old new] arg).run (terminates_star.mpr term)
+      = let res := new ++ arg ++ (old.pmap (fun ent rt ↦ if h : s < ent.1
+          then [/⟨r⟩*‹t›/].matchPartial w ent.1 ent.2 (rt h)
+          else [ent]) term).flatten;
+        match (generalizing := false) t with
+        | .greedy => res ++ [(s, cap)]
+        | .lazy => [(s, cap)] ++ res := by
+  induction old generalizing new arg with
+  | nil => step; step; rfl
+  | cons ent mat ind =>
+    simp only [List.mem_cons, forall_eq_or_imp, List.pmap_cons,
+      List.flatten_cons] at term ⊢
+    simp only at ind
+    step
+    split <;> rename_i hs
+    · run_top!
+      rw [ind term.2]
+      simp; rfl
+    · rw [ind term.2]
+      simp
+
+theorem Action.starWait_run {t : StarType} {arg : PartialMatches w}
+    (term : ∀ mat ∈ arg, s < mat.1 → [/⟨r⟩*‹t›/].Terminates w mat.1 mat.2)
+    : (mk [.starWait t r s cap] arg).run (terminates_starWait.mpr term)
+      = let res := (arg.pmap (fun ent rt ↦ if h : s < ent.1
+          then [/⟨r⟩*‹t›/].matchPartial w ent.1 ent.2 (rt h)
+          else [ent]) term).flatten;
+        match (generalizing := false) t with
+        | .greedy => res ++ [(s, cap)]
+        | .lazy => [(s, cap)] ++ res := by
   step only [List.append_nil]
-  cases t with
-  | greedy =>
-    simp only
-    rw [← matchPartial_terminates_iff, terminates_or,
-      terminates_or] at ⊢
-    rw! [terminates_filterEmpty, terminates_concat,
-      terminates_filterEmpty]
-    simp [terminates_empty, matchPartial_filterEmpty]
-  | lazy =>
-    simp only
-    rw [← matchPartial_terminates_iff, terminates_or,
-      terminates_or] at ⊢
-    rw! [terminates_filterEmpty, terminates_concat,
-      terminates_filterEmpty]
-    simp [terminates_empty, matchPartial_filterEmpty]
+  exact star_run term
 
 theorem matchPartial_star {t : StarType}
     (term : [/⟨r⟩*‹t›/].Terminates w s cap)
-    : matchPartial [/⟨r⟩*‹t›/] w s cap term = match t with
-      | .greedy => [/(⟨r⟩ •ε | (⟨r⟩ -ε) ⟨r⟩*) | ε/].matchPartial w s cap
-        (matchPartial_star_greedy_terminates'.mp term)
-      | .lazy => [/ε | (⟨r⟩ •ε | (⟨r⟩ -ε) ⟨r⟩*?)/].matchPartial w s cap
-        (matchPartial_star_lazy_terminates'.mp term)
-      := by
-  simp only [matchPartial_eq_run]
-  split <;> conv_lhs => step
+    : matchPartial [/⟨r⟩*‹t›/] w s cap term =
+      let res := ((r.matchPartial w s cap (terminates_star.mp term).1).pmap
+        (fun ent rt ↦ if h : s < ent.1
+          then [/⟨r⟩*‹t›/].matchPartial w ent.1 ent.2 (rt h)
+          else [ent]) (terminates_star.mp term).2).flatten;
+      match (generalizing := false) t with
+      | .greedy => res ++ [(s, cap)]
+      | .lazy => [(s, cap)] ++ res := by
+  rw [matchPartial]
+  simp only [initMatchPartial]
+  step
+  run_top!
+  rw! [← matchPartial_eq_run]
+  rw [Action.starWait_run (terminates_star.mp term).2]
+  rfl
 
 theorem matchPartial_start
     : matchPartial [/⊢/] w s cap terminates_start
@@ -450,13 +513,13 @@ theorem matchPartial_end'
       = if s = w.length then [(s, cap)] else [] := by
   simp only [matchPartial_eq_run]; step; step
 
-theorem Action.capture_run {n : ℕ} {arg : PartialMatches}
+theorem Action.capture_run {n : ℕ} {arg : PartialMatches w}
     : (mk [.capture (α := α) n s] arg).run terminates_capture
       = arg.map fun ent ↦ (ent.1, ent.2.update n [(s, ent.1)]) := by step; step
 
 theorem matchPartial_capture {n : ℕ}
-    (term : [/(‹n› ⟨r⟩)/].Terminates w s cap)
-    : matchPartial [/(‹n› ⟨r⟩)/] w s cap term =
+    (term : [/(n ← ⟨r⟩)/].Terminates w s cap)
+    : matchPartial [/(n ← ⟨r⟩)/] w s cap term =
       (r.matchPartial w s cap (terminates_capture.mp term)).map
         fun ent ↦ (ent.1, ent.2.update n [(s, ent.1)]) := by
   rw [matchPartial]
@@ -467,14 +530,15 @@ theorem matchPartial_capture {n : ℕ}
   rfl
 
 /-- `list` always terminates -/
-theorem list_terminates {l : List α}
+theorem terminates_list {l : List α}
     : (list l).Terminates w s cap := by
   induction l generalizing s with
   | nil => rw [list]; exact terminates_empty
   | cons a as ind =>
     rw [list, terminates_concat]
-    simp only [matchPartial_unit, List.mem_ite_nil_right, List.mem_cons, List.not_mem_nil, or_false,
-      and_imp, forall_eq_apply_imp_iff, terminates_unit, exists_const]
+    simp only [matchPartial_unit, List.mem_dite_nil_right, List.mem_cons,
+      List.not_mem_nil, or_false, forall_exists_index, forall_eq_apply_imp_iff, terminates_unit,
+      exists_const]
     exact fun _ ↦ ind
 
 /-- `backref` always terminates -/
@@ -484,18 +548,21 @@ theorem terminates_backref {d : BackrefDefault} {n : ℕ}
   step
   split <;> expose_names
   · split <;> (step; step)
-  exact list_terminates
+  exact terminates_list
 
 theorem matchPartial_list {l : List α}
-    : matchPartial (list l) w s cap list_terminates =
-    if w.extract s (s + l.length) = l then [(s + l.length, cap)] else [] := by
+    : matchPartial (list l) w s cap terminates_list =
+    if h : w.extract s (s + l.length) = l then [(s.addOfIndex h rfl, cap)] else [] := by
   induction l generalizing s with
-  | nil => simp [list, matchPartial_empty]
+  | nil => simp [← Fin.val_inj, list, matchPartial_empty]
   | cons a as ind =>
     simp only [list, matchPartial_concat, List.length_cons, matchPartial_unit]
-    by_cases! h : w[s]? = a
-    · specialize ind (s := s + 1)
-      simp only [h, ↓reduceIte, List.pmap_cons, ind,
+    by_cases! h : w[s.val]? = a
+    · specialize ind (s := s.succOfIndex h)
+      --simp only [Pos.val_succOfIndex] at ind
+      rw! [Pos.val_succOfIndex] at ind
+      simp only at ind
+      simp only [h, ↓reduceDIte, List.pmap_cons, ind,
         List.pmap_nil, List.flatten_cons, List.flatten_nil, List.append_nil]
       rw! [← add_assoc, add_right_comm]
       have eq : (w.extract (s + 1) (s + as.length + 1) = as)
@@ -506,9 +573,10 @@ theorem matchPartial_list {l : List α}
         have ⟨lt, wsa⟩ := List.getElem?_eq_some_iff.mp h
         conv_rhs => rw [List.drop_eq_getElem_cons lt, List.take_cons (by linarith), wsa]
         simp
-      simp only [eq]
-    simp only [h, ↓reduceIte, List.pmap_nil, List.flatten_nil, List.extract_eq_drop_take,
-      add_tsub_cancel_left, right_eq_ite_iff, List.ne_cons_self, imp_false]
+      rw! (castMode := .all) [eq]
+      split <;> simp [← Fin.val_inj, add_assoc, add_comm 1]
+    simp only [h, ↓reduceDIte, List.pmap_nil, List.flatten_nil, List.extract_eq_drop_take,
+      add_tsub_cancel_left, right_eq_dite_iff, List.ne_cons_self, imp_false]
     by_cases! h' : s < w.length
     · contrapose! h
       rw [List.drop_eq_getElem_cons h', List.take_cons (by linarith)] at h
@@ -520,8 +588,8 @@ theorem matchPartial_backref {n : ℕ} {d : BackrefDefault}
     : matchPartial [/\‹d›n/] w s cap terminates_backref =
       match (cap n).head? with
       | none => match d with | .bot => [] | .empty => [(s, cap)]
-      | some (cs, ct) => if w.extract s (s + (w.extract cs ct).length) = w.extract cs ct
-        then [(s + (w.extract cs ct).length, cap)]
+      | some (cs, ct) => if h : w.extract s (s + (ct - cs)) = w.extract cs ct
+        then [(s.addOfIndex h (List.length_extract_pos _ _), cap)]
         else [] := by
   rw [matchPartial_eq_run]
   step only [List.append_nil]
@@ -531,7 +599,7 @@ theorem matchPartial_backref {n : ℕ} {d : BackrefDefault}
   · simp only [← heeq, h]
     split <;> (step; step)
   · simp only [← heeq, h]
-    rw! [← matchPartial_eq_run, matchPartial_list]
+    rw! [← matchPartial_eq_run, matchPartial_list, List.length_extract_pos]
     rfl
 
 end MatchPartial
