Regex/Match.lean
@@ -1,132 +1,14 @@
 import Regex.Basic
-import Regex.Lemmas.Bounds
+import Regex.Lemmas.Mem
 
 namespace Regex
 variable {α : Type u} [deq : DecidableEq α] {r : Regex α} {w : List α}
-
-/-- Convenience theorem for membership of a star match, as suggested by `simp` -/
-theorem mem_matchPartial_star {t : StarType} {s} {cap}
-    (term : [/⟨r⟩*‹t›/].Terminates w s cap) (mat)
-    : mat ∈ [/⟨r⟩*‹t›/].matchPartial w s cap term ↔
-      mat ∈ r.matchPartial w s cap (terminates_star.mp term).1 ∧ mat.1 ≤ s ∨
-      (∃ (mid : _) (mem : mid ∈ r.matchPartial w s cap (terminates_star.mp term).1 ∧
-        s < mid.1), mat ∈ [/⟨r⟩*/].matchPartial w mid.1 mid.2
-          (terminates_star_iff_greedy.mp ((terminates_star.mp term).2 _ mem.1 mem.2))) ∨
-      mat = (s, cap) := by
-  revert term; rw! [terminates_star_iff_greedy]; intro term
-  rw [mem_matchPartial_star_iff_greedy]
-  rw [matchPartial_star]
-  simp [matchPartial_or, matchPartial_filterEmpty, matchPartial_concat,
-    matchPartial_empty]
-
-private theorem mem_matchPartial_star'α {t : StarType} {s} {cap}
-    (term : [/⟨r⟩*‹t›/].Terminates w s cap) {mat}
-    : mat ∈ [/⟨r⟩*‹t›/].matchPartial w s cap term →
-      ∃ (ls : List (ℕ × Captures)) (nemp : ls ≠ []),
-        ls.head nemp = (s, cap) ∧ ls.getLast nemp = mat ∧
-        ∀ (i : _) (h : i + 1 < ls.length),
-          ∃ term' : r.Terminates w ls[i].1 ls[i].2,
-          ls[i + 1] ∈ r.matchPartial w ls[i].1 ls[i].2 term' ∧
-          (i + 2 = ls.length ∨ ls[i].1 < ls[i + 1].1) := by
-  revert term; rw! [terminates_star_iff_greedy]; intro term
-  rw [mem_matchPartial_star_iff_greedy]
-  by_cases! sle : s ≤ w.length
-  · induction s, sle using decreasingStrongRec generalizing cap mat with | ind s sle ind =>
-      rw [mem_matchPartial_star]
-      rintro (mem | ⟨mid, mem, mem'⟩ | eq)
-      · use [(s, cap), mat]
-        simp only [List.head_cons, ne_eq, List.cons_ne_self, not_false_eq_true, List.getLast_cons,
-          List.getLast_singleton, List.length_cons, List.length_nil, zero_add, Nat.reduceAdd,
-          List.getElem_cons_succ, List.getElem_singleton, true_and, reduceCtorEq, exists_const]
-        intro i i0
-        simp only [show i = 0 by linarith, List.getElem_cons_zero, zero_add, true_or, and_true]
-        exact ⟨(terminates_star.mp term).1, mem.1⟩
-      · have ⟨ls', nemp', fst', lst', conn'⟩ :=
-          ind _ (endInBounds _ _ sle _ _ _ mem.1) mem.2
-          ((terminates_star.mp term).2 _ mem.1 mem.2) mem'
-        use (s, cap) :: ls'
-        simp only [List.head_cons, List.getLast_cons nemp', lst', List.length_cons,
-          Order.lt_add_one_iff, Order.add_one_le_iff, Nat.reduceEqDiff, List.getElem_cons_succ,
-          true_and, ne_eq, reduceCtorEq, not_false_eq_true, exists_const]
-        intro i ilt
-        cases i with
-        | zero => simp [List.getElem_zero_eq_head, fst', (terminates_star.mp term).1, mem]
-        | succ i =>
-          specialize conn' i ilt
-          simp only [List.getElem_cons_succ]
-          exact conn'
-      · use [(s, cap)]; simp [eq]
-  · rw [mem_matchPartial_star]
-    rintro (mem | ⟨mid, mem, mem'⟩ | eq)
-    · use [(s, cap), mat]
-      simp only [List.head_cons, ne_eq, List.cons_ne_self, not_false_eq_true, List.getLast_cons,
-        List.getLast_singleton, List.length_cons, List.length_nil, zero_add, Nat.reduceAdd,
-        Nat.add_eq_right, List.getElem_cons_succ, List.getElem_singleton, true_and, reduceCtorEq,
-        exists_const]
-      intro i i0
-      simp only [show i = 0 by linarith, List.getElem_cons_zero, true_or, and_true]
-      exact ⟨(terminates_star.mp term).1, mem.1⟩
-    · have bound := matchPartial_outOfBounds_eq (le_of_lt sle) mem.1; simp [bound] at mem
-    · use [(s, cap)]; simp [eq]
-
-private theorem mem_matchPartial_star'β {t : StarType} {s} {cap}
-    (term : [/⟨r⟩*‹t›/].Terminates w s cap) {mat}
-    : (∃ (ls : List (ℕ × Captures)) (nemp : ls ≠ []),
-        ls.head nemp = (s, cap) ∧ ls.getLast nemp = mat ∧
-        ∀ (i : _) (h : i + 1 < ls.length),
-          ∃ term' : r.Terminates w ls[i].1 ls[i].2,
-          ls[i + 1] ∈ r.matchPartial w ls[i].1 ls[i].2 term' ∧
-          (i + 2 = ls.length ∨ ls[i].1 < ls[i + 1].1)) →
-      mat ∈ [/⟨r⟩*‹t›/].matchPartial w s cap term := by
-  revert term; rw! [terminates_star_iff_greedy]; intro term
-  rw [mem_matchPartial_star_iff_greedy]
-  rintro ⟨ls, nemp, fst, lst, conn⟩
-  induction ls generalizing s cap mat <;> try contradiction
-  rename_i l ls ind
-  rw [mem_matchPartial_star]
-  cases ls with
-  | nil =>
-    rw [List.head_singleton] at fst
-    simp [fst] at lst
-    simp [lst]
-  | cons l' ls =>
-    simp only [ne_eq, reduceCtorEq, not_false_eq_true, List.head_cons, List.length_cons,
-      Order.lt_add_one_iff, Order.add_one_le_iff, Nat.reduceEqDiff, List.getElem_cons_succ,
-      forall_true_left, Prod.forall, List.getLast_cons, add_le_add_iff_right,
-      Nat.add_right_cancel_iff] at ind fst lst conn
-    have conn0 := conn 0 (Nat.zero_le _)
-    simp only [List.getElem_cons_zero, exists_and_right, fst] at conn0
-    have ⟨⟨term', mem⟩, zeq⟩ := conn0
-    by_cases! l'le : l'.1 ≤ s
-    · simp only [not_lt.mpr l'le, or_false] at zeq
-      rw [eq_comm, ← List.eq_nil_iff_length_eq_zero] at zeq
-      simp only [zeq, List.getLast_singleton] at lst
-      exact Or.inl ⟨lst ▸ mem, lst ▸ l'le⟩
-    have term'' := (terminates_star.mp term).2 _ mem l'le
-    specialize ind _ _ term'' rfl lst _
-    · intro i ilt
-      specialize conn (i + 1) (by linarith)
-      simp only [List.getElem_cons_succ, exists_and_right] at conn ⊢
-      exact conn
-    exact Or.inr (Or.inl ⟨_, ⟨mem, l'le⟩, ind⟩)
-
-/-- Non-recursive version of membership of a star match -/
-theorem mem_matchPartial_star' {t : StarType} {s} {cap}
-    (term : [/⟨r⟩*‹t›/].Terminates w s cap) {mat}
-    : mat ∈ [/⟨r⟩*‹t›/].matchPartial w s cap term ↔
-      ∃ (ls : List (ℕ × Captures)) (nemp : ls ≠ []),
-        ls.head nemp = (s, cap) ∧ ls.getLast nemp = mat ∧
-        ∀ (i : _) (h : i + 1 < ls.length),
-          ∃ term' : r.Terminates w ls[i].1 ls[i].2,
-          ls[i + 1] ∈ r.matchPartial w ls[i].1 ls[i].2 term' ∧
-          (i + 2 = ls.length ∨ ls[i].1 < ls[i + 1].1) :=
-  ⟨mem_matchPartial_star'α term, mem_matchPartial_star'β term⟩
 
 /-! Stuff about full matches -/
 
 /-- Returns all matches that end at the end of the string -/
 def match' (r : Regex α) (w : List α) (term : r.Terminates w 0 0) :
-  PartialMatches := [/⟨r⟩ ⊣/].matchPartial w 0 0
+  PartialMatches w := [/⟨r⟩ ⊣/].matchPartial w 0 0
     (terminates_concat.mpr ⟨term, fun _ _ ↦ terminates_end'⟩)
 
 theorem match'_def (term : r.Terminates w 0 0)
@@ -144,8 +26,8 @@ theorem mem_match'_iff (term : r.Terminates w 0 0) {mat}
 
 /-- The condition specialized for (w.length, cap) -/
 theorem mem_match'_iff_length_mem (term : r.Terminates w 0 0) {cap}
-    : (w.length, cap) ∈ r.match' w term ↔
-      (w.length, cap) ∈ r.matchPartial w 0 0 term := by
+    : (Fin.last w.length, cap) ∈ r.match' w term ↔
+      (Fin.last w.length, cap) ∈ r.matchPartial w 0 0 term := by
   simp [mem_match'_iff]
 
 /-- Returns whether the whole sequence matches the regex.
@@ -162,13 +44,14 @@ theorem isMatch_bot : ¬[/⊥/].IsMatch w terminates_bot := by
 theorem isMatch_empty : [//].IsMatch w terminates_empty ↔ w = [] := by
   simp only [IsMatch, match'_def, matchPartial_empty, ne_eq, List.filter_eq_nil_iff, List.mem_cons,
     List.not_mem_nil, or_false, decide_eq_true_eq, forall_eq, Decidable.not_not]
-  rw [eq_comm, List.length_eq_zero_iff]
+  rw [eq_comm, Fin.val_zero, List.length_eq_zero_iff]
 
 /-- A unit regex matches only the singleton sequence that has that unit -/
 theorem isMatch_unit {c : α} : [/`‹c›/].IsMatch w terminates_unit ↔ w = [c] := by
-  simp only [IsMatch, match'_def, matchPartial_unit, zero_add, ne_eq, List.filter_eq_nil_iff,
-    List.mem_ite_nil_right, List.mem_cons, List.not_mem_nil, or_false, decide_eq_true_eq, and_imp,
-    forall_eq_apply_imp_iff, Classical.not_imp, Decidable.not_not]
+  simp only [IsMatch, match'_def, matchPartial_unit, Fin.coe_ofNat_eq_mod, Nat.zero_mod, ne_eq,
+    List.filter_eq_nil_iff, List.mem_dite_nil_right, List.mem_cons, List.not_mem_nil, or_false,
+    decide_eq_true_eq, forall_exists_index, forall_eq_apply_imp_iff, Pos.val_succOfIndex, zero_add,
+    Classical.not_imp, Decidable.not_not]
   rw [eq_comm (a := 1), List.length_eq_one_iff, List.getElem?_eq_some_iff]
   constructor
   · rintro ⟨⟨lt, eqc⟩, ⟨c', eqc'⟩⟩
@@ -196,70 +79,26 @@ theorem isMatch_star {t : StarType} {r : Regex α} (term : [/⟨r⟩*‹t›/].T
     : [/⟨r⟩*‹t›/].IsMatch w term ↔
       w = [] ∨
       ∃ (mat : _) (mem : mat ∈ r.matchPartial w 0 0 (terminates_star.mp term).1)
-        (lt : 0 < mat.1), ∃ mat' ∈ [/⟨r⟩*/].matchPartial w mat.1 mat.2
-          (terminates_star_iff_greedy.mp ((terminates_star.mp term).2 _ mem lt)),
-          mat'.1 = w.length := by
-  simp only [IsMatch, match'_def, ne_eq, List.filter_eq_nil_iff, decide_eq_true_eq, Prod.forall,
-    not_forall, Decidable.not_not, exists_and_right, exists_eq_right, Prod.exists]
-  simp only [exists_prop, exists_and_right, exists_eq_right]
-  conv in _ ∈ _ => rw [mem_matchPartial_star_iff_greedy]
-  rw [matchPartial_star]
-  simp only [matchPartial_or, matchPartial_filterEmpty, ge_iff_le, nonpos_iff_eq_zero, eq_iff_iff,
-    iff_true, matchPartial_concat, Bool.false_eq_true, iff_false, decide_not, matchPartial_empty,
-    List.append_assoc, List.mem_append, List.mem_filter, List.length_eq_zero_iff, decide_eq_true_eq,
-    List.mem_flatten, List.mem_pmap, Bool.not_eq_eq_eq_not, Bool.not_true, decide_eq_false_iff_not,
-    Prod.exists, ↓existsAndEq, true_and, List.mem_cons, Prod.mk.injEq, List.not_mem_nil, or_false]
+        (lt : 0 < mat.1), ∃ mat' ∈ [/⟨r⟩*‹t›/].matchPartial w mat.1 mat.2
+          ((terminates_star.mp term).2 _ mem lt),
+        mat'.1 = w.length := by
+  simp only [IsMatch, match'_def, ne_eq, List.filter_eq_nil_iff, decide_eq_true_eq,
+    not_forall, Decidable.not_not]
+  conv => enter [1, 1, x]; rw [mem_matchPartial_star]
   constructor
-  · rintro ⟨cap', mem | ⟨s, cap, mem, mem'⟩ | eq⟩
-    · simp [mem]
-    · exact Or.inr ⟨_, _, mem.1, Nat.pos_iff_ne_zero.mpr mem.2, _, mem'⟩
-    · simp [eq]
-  · rintro (eq | ⟨s, cap, mem, lt, cap', mem'⟩)
-    · exact ⟨0, Or.inr (Or.inr ⟨eq, rfl⟩)⟩
-    · exact ⟨cap', Or.inr (Or.inl ⟨_, _, ⟨mem, Nat.pos_iff_ne_zero.mp lt⟩, mem'⟩)⟩
-
-theorem isMatch_star_greedy_iff_lazy
-    {r : Regex α} (term : [/⟨r⟩*/].Terminates w 0 0)
-    : [/⟨r⟩*/].IsMatch w term ↔ [/⟨r⟩*?/].IsMatch w
-      (terminates_star_greedy_iff_lazy.mp term) := by
-  rw [isMatch_star, ← isMatch_star (t := .lazy)];
-
-theorem isMatch_star_iff_greedy {t : StarType}
-    {r : Regex α} (term : [/⟨r⟩*‹t›/].Terminates w 0 0)
-    : [/⟨r⟩*‹t›/].IsMatch w term ↔ [/⟨r⟩*/].IsMatch w (terminates_star_iff_greedy.mp term) := by
-  cases t <;> simp [isMatch_star_greedy_iff_lazy]
-
-theorem isMatch_star_iff_lazy {t : StarType}
-    {r : Regex α} (term : [/⟨r⟩*‹t›/].Terminates w 0 0)
-    : [/⟨r⟩*‹t›/].IsMatch w term ↔ [/⟨r⟩*?/].IsMatch w (terminates_star_iff_lazy.mp term) := by
-  cases t <;> simp [isMatch_star_greedy_iff_lazy]
-
-/-- Non-recursive version, stated with a nonempty list -/
-theorem isMatch_star' {t : StarType} {r : Regex α} (term : [/⟨r⟩*‹t›/].Terminates w 0 0)
-    : [/⟨r⟩*‹t›/].IsMatch w term ↔
-      ∃ (ls : List (ℕ × Captures)) (nemp : ls ≠ []),
-        ls.head nemp = (0, 0) ∧ (ls.getLast nemp).1 = w.length ∧
-        ∀ (i : _) (h : i + 1 < ls.length),
-          ∃ term' : r.Terminates w ls[i].1 ls[i].2,
-          ls[i + 1] ∈ r.matchPartial w ls[i].1 ls[i].2 term' ∧
-          (i + 2 = ls.length ∨ ls[i].1 < ls[i + 1].1) := by
-  rw [IsMatch, match'_def, ne_eq, List.filter_eq_nil_iff]
-  conv in _ ∈ _ => rw [mem_matchPartial_star']
-  push_neg
-  conv in (∃ _, _) ∧ _ => rw [← exists_and_right]
-  conv in (∃ _, _) ∧ _ => rw [← exists_and_right]
-  -- conv stopped working with unknown goal _uniq.321197
-  simp only [and_assoc (c := decide _ = _), and_comm (b := decide _ = _)]
-  simp
-
-theorem decide_eq_bool {p : Prop} [Decidable p] {b : Bool}
-    : decide p = b ↔ (p ↔ b = true) := by cases b <;> simp
-
-theorem isMatch_filterEmpty {e : Bool} {r : Regex α}
-    (term : [/⟨r⟩ ‹e›ε/].Terminates w 0 0)
-    : [/⟨r⟩ ‹e›ε/].IsMatch w term ↔
-      r.IsMatch w (terminates_filterEmpty.mp term) ∧ (w.length = 0) = e := by
-  simp [IsMatch, match'_def, matchPartial_filterEmpty, decide_eq_bool]
+  · rintro ⟨mat, zero | ⟨mid, mem, mem'⟩, len⟩
+    · rw [List.eq_nil_iff_length_eq_zero]
+      simp [← len]; simp [zero]
+    · split at mem' <;> expose_names
+      · grind
+      · simp only [not_lt, Fin.le_zero_iff] at h
+        rw [List.eq_nil_iff_length_eq_zero]
+        simp [← len, mem']; simp [h]
+  · rintro (emp | ⟨mid, mem, lt, mat, mem', len⟩)
+    · use (0, 0)
+      rw [List.eq_nil_iff_length_eq_zero] at emp
+      simp [emp]
+    · grind
 
 -- Some silly ones
 
@@ -267,18 +106,18 @@ theorem isMatch_filterEmpty {e : Bool} {r : Regex α}
 theorem isMatch_start : [/⊢/].IsMatch w terminates_start ↔ w = [] := by
   simp only [IsMatch, match'_def, matchPartial_start, ↓reduceIte, ne_eq, List.filter_eq_nil_iff,
     List.mem_cons, List.not_mem_nil, or_false, decide_eq_true_eq, forall_eq, Decidable.not_not]
-  rw [eq_comm, List.length_eq_zero_iff]
+  rw [eq_comm, Fin.val_zero, List.length_eq_zero_iff]
 
 /-- The end anchor full-matches only the empty sequence -/
 theorem isMatch_end' : [/⊣/].IsMatch w terminates_end' ↔ w = [] := by
   simp only [IsMatch, match'_def, matchPartial_end', ne_eq, List.filter_eq_nil_iff,
     List.mem_ite_nil_right, List.mem_cons, List.not_mem_nil, or_false, decide_eq_true_eq, and_imp,
     forall_eq_apply_imp_iff, imp_not_self, Decidable.not_not]
-  rw [eq_comm, List.length_eq_zero_iff]
+  rw [eq_comm, Fin.val_zero, List.length_eq_zero_iff]
 
 /-- A capture of `r` matches iff `r` matches -/
-theorem isMatch_capture {n : ℕ} {r : Regex α} (term : [/(‹n› ⟨r⟩)/].Terminates w 0 0)
-    : [/(‹n› ⟨r⟩)/].IsMatch w term ↔ r.IsMatch w (terminates_capture.mp term) := by
+theorem isMatch_capture {n : ℕ} {r : Regex α} (term : [/(n ← ⟨r⟩)/].Terminates w 0 0)
+    : [/(n ← ⟨r⟩)/].IsMatch w term ↔ r.IsMatch w (terminates_capture.mp term) := by
   simp [IsMatch, match'_def, matchPartial_capture]
 
 /-- A full-match on a backref just defaults -/
@@ -287,7 +126,7 @@ theorem isMatch_backref {d : BackrefDefault} {n : ℕ}
         | .bot => False
         | .empty => w = [] := by
   simp [IsMatch, match'_def, matchPartial_backref]
-  split <;> simp
+  split <;> simp [← List.length_eq_zero_iff, eq_comm]
 
 /-- The language of a regex is the set of languages that it full-matches. -/
 def language (r : Regex α) (term : ∀ w, r.Terminates w 0 0)
@@ -327,28 +166,18 @@ theorem language_or {q r : Regex α} (term : ∀ w, [/⟨q⟩ | ⟨r⟩/].Termin
       r.language (fun _ ↦ (terminates_or.mp (term _)).2) := by
   simp [language, isMatch_or, Language.add_def, Set.union_def]
 
-theorem language_filterEmpty {e : Bool} {r : Regex α}
-    (term : ∀ w, [/⟨r⟩ ‹e›ε/].Terminates w 0 0)
-    : ([/⟨r⟩ ‹e›ε/] : Regex α).language term = if e then
-        r.language (fun _ ↦ terminates_filterEmpty.mp (term _)) ⊓ {[]} else
-        r.language (fun _ ↦ terminates_filterEmpty.mp (term _)) - {[]} := by
-  simp only [language, isMatch_filterEmpty, List.length_eq_zero_iff, eq_iff_iff]
-  split <;> (expose_names; simp only [h, iff_true, Bool.false_eq_true, iff_false])
-  · ext x; rw [Language.mem_inf, Set.setOf_and, Set.mem_inter_iff]; rfl
-  · ext x; rw [Language.mem_sub, Set.setOf_and, Set.mem_inter_iff]; rfl
-
 /-- Not a simple language description, but this is the language of a star.
 Note that it is *not* the star of the individual language. -/
 theorem language_star {t : StarType} {r : Regex α}
     (term : ∀ w, [/⟨r⟩*‹t›/].Terminates w 0 0)
     : [/⟨r⟩*‹t›/].language term =
-      {w | ∃ (ls : List (ℕ × Captures)) (nemp : ls ≠ []),
-        ls.head nemp = (0, 0) ∧ (ls.getLast nemp).1 = w.length ∧
-        ∀ (i : _) (h : i + 1 < ls.length),
-          ∃ term' : r.Terminates w ls[i].1 ls[i].2,
-          ls[i + 1] ∈ r.matchPartial w ls[i].1 ls[i].2 term' ∧
-          (i + 2 = ls.length ∨ ls[i].1 < ls[i + 1].1)} := by
-  simp [language, isMatch_star']
+      {[]} ∪ {w | ∃ (mat : _)
+        (mem : mat ∈ r.matchPartial w 0 0 (terminates_star.mp (term w)).1)
+        (lt : 0 < mat.1), ∃ mat' ∈ [/⟨r⟩*‹t›/].matchPartial w mat.1 mat.2
+          ((terminates_star.mp (term w)).2 _ mem lt),
+        mat'.1 = w.length} := by
+  simp [language, isMatch_star]
+  simp [Set.insert_def]
 
 theorem language_start : ([/⊢/] : Regex α).language (fun _ ↦ terminates_start) = {[]} := by
   simp [language, isMatch_start]
@@ -356,8 +185,8 @@ theorem language_start : ([/⊢/] : Regex α).language (fun _ ↦ terminates_sta
 theorem language_end' : ([/⊣/] : Regex α).language (fun _ ↦ terminates_end') = {[]} := by
   simp [language, isMatch_end']
 
-theorem language_capture {n : ℕ} {r : Regex α} (term : ∀ w, [/(‹n› ⟨r⟩)/].Terminates w 0 0)
-    : ([/(‹n› ⟨r⟩)/] : Regex α).language term =
+theorem language_capture {n : ℕ} {r : Regex α} (term : ∀ w, [/(n ← ⟨r⟩)/].Terminates w 0 0)
+    : ([/(n ← ⟨r⟩)/] : Regex α).language term =
       r.language (fun _ ↦ terminates_capture.mp (term _)) := by
   simp [language, isMatch_capture]
 
