Regex/Termination.lean
@@ -1,8 +1,21 @@
-import Regex.Lemmas.Bounds
+import Regex.Basic
 
 namespace Regex
 
 variable {α : Type u} [deq : DecidableEq α] {r : Regex α} {w : List α}
+  {s : Pos w} {cap : Captures w}
+
+/-- `star t r` terminates if (but not only if)
+`r` terminates for every capture and for every position starting from here -/
+theorem terminates_star_of_forall {t : StarType}
+    : (∀ s' ≥ s, ∀ cap', r.Terminates w s' cap') →
+      [/⟨r⟩*‹t›/].Terminates w s cap := by
+  intro term
+  induction s using Pos.strongRecEnd generalizing cap with
+  | ind s ind =>
+    rw [terminates_star]
+    refine ⟨term s (le_refl _) cap, fun mat mem lt ↦ ?_⟩
+    exact ind mat.1 lt (fun s' ge ↦ term s' (le_of_lt (Trans.trans lt ge)))
 
 section Tactic
 
@@ -11,7 +24,7 @@ open Lean Parser Tactic
 macro "termination" : tactic =>
   `(tactic| (repeat simp [
     terminates_bot, terminates_empty, terminates_unit, terminates_concat,
-    terminates_or, terminates_filterEmpty, terminates_start, terminates_end',
+    terminates_or, terminates_start, terminates_end',
     terminates_capture, terminates_backref, terminates_star_of_forall];
     ))
 
@@ -43,19 +56,14 @@ theorem allTerminates_or_comm {q r : Regex α}
     : [/⟨q⟩ | ⟨r⟩/].AllTerminates ↔ [/⟨r⟩ | ⟨q⟩/].AllTerminates := by
   simp only [AllTerminates, terminates_or_comm (q := q)]
 
-theorem allTerminates_filterEmpty {e : Bool} {r : Regex α}
-    (rt : r.AllTerminates)
-    : [/⟨r⟩ ‹e›ε/].AllTerminates (α := α) :=
-  fun w s cap ↦ terminates_filterEmpty.mpr (rt w s cap)
-
 theorem allTerminates_star {t : StarType} {r : Regex α}
     (rt : r.AllTerminates)
     : [/⟨r⟩*‹t›/].AllTerminates (α := α) :=
   fun w _ _ ↦ terminates_star_of_forall fun s' _ cap' ↦ rt w s' cap'
 
-theorem allTerminates_star_greedy_iff_lazy {r : Regex α}
-    : [/⟨r⟩*/].AllTerminates ↔ [/⟨r⟩*?/].AllTerminates := by
-  simp only [AllTerminates, terminates_star_greedy_iff_lazy]
+--theorem allTerminates_star_greedy_iff_lazy {r : Regex α}
+--    : [/⟨r⟩*/].AllTerminates ↔ [/⟨r⟩*?/].AllTerminates := by
+--  simp only [AllTerminates, terminates_star_greedy_iff_lazy]
 
 theorem allTerminates_start : [/⊢/].AllTerminates (α := α) :=
   fun _ _ _ ↦ terminates_start
@@ -65,7 +73,7 @@ theorem allTerminates_end' : [/⊣/].AllTerminates (α := α) :=
 
 theorem allTerminates_capture {n : ℕ} {r : Regex α}
     (rt : r.AllTerminates)
-    : [/(‹n› ⟨r⟩)/].AllTerminates (α := α) :=
+    : [/(n ← ⟨r⟩)/].AllTerminates (α := α) :=
   fun w s cap ↦ terminates_capture.mpr (rt w s cap)
 
 theorem allTerminates_backref {d : BackrefDefault} {n : ℕ}
@@ -78,7 +86,6 @@ inductive CTerminates : Regex α → Prop where
   | unit c : CTerminates (unit c)
   | concat q r : CTerminates q → CTerminates r → CTerminates (concat q r)
   | or q r : CTerminates q → CTerminates r → CTerminates (or q r)
-  | filterEmpty e r : CTerminates r → CTerminates (filterEmpty e r)
   | star t r : CTerminates r → CTerminates (star t r)
   | start : CTerminates start
   | end' : CTerminates end'
@@ -95,13 +102,12 @@ theorem CTerminates.allTerminates {r : Regex α} (hr : r.CTerminates)
   | unit c => termination
   | concat q r _ _ qt rt => simp [terminates_concat, qt, rt]
   | or q r _ _ qt rt => simp [terminates_or, qt, rt]
-  | filterEmpty e r _ rt => simp [terminates_filterEmpty, rt]
   | star t r _ rt => intro r s cap; apply terminates_star_of_forall; simp [rt]
   | start => termination
   | end' => termination
   | capture n r _ rt => simp [terminates_capture, rt]
   | backref d n => termination
 
-#eval [/(‹0› (0 | ε)*)/].matchPartial [0] 0 0 (by termination)
+--#eval [/(0 ← (0 | ε)*)/].matchPartial [0] 0 0 (by termination)
 
 end Regex
