Regex/Lemmas/Equiv.lean
@@ -1,0 +1,331 @@
+import Regex.Basic
+import Regex.Termination
+import Regex.Lemmas.Mem
+import Regex.Match
+
+namespace Regex
+
+variable {α : Type u} [deq : DecidableEq α] {q r : Regex α} {w : List α}
+  {s : Pos w} {cap : Captures w}
+
+/-- Whether two regexes are terminates-equivalent.
+If two regexes are weakly matchPartial-equivalent, you can replace a
+termination predicate in one regex with the other. -/
+def TerminatesEquiv (q r : Regex α) :=
+  ∀ w s cap, q.Terminates w s cap ↔ r.Terminates w s cap
+
+@[inherit_doc]
+scoped notation:25 q:25 " ≃ᵗᵉ " r:26 => TerminatesEquiv q r
+
+namespace TerminatesEquiv
+
+@[refl] theorem refl (r : Regex α) : r ≃ᵗᵉ r := by simp [TerminatesEquiv]
+
+@[symm] theorem symm {q r : Regex α} (qr : q ≃ᵗᵉ r) : r ≃ᵗᵉ q := by
+  simp [TerminatesEquiv] at qr ⊢; simp [qr]
+
+@[trans] theorem trans {p q r : Regex α} (pq : p ≃ᵗᵉ q) (qr : q ≃ᵗᵉ r)
+    : p ≃ᵗᵉ r := by
+  simp [TerminatesEquiv] at pq qr ⊢; simp [pq, qr]
+
+theorem allTerminates (heq : q ≃ᵗᵉ r) : q.AllTerminates ↔ r.AllTerminates := by
+  rw [TerminatesEquiv] at heq
+  simp only [AllTerminates]
+  grind
+
+end TerminatesEquiv
+
+theorem terminatesEquiv_bot_concat {r : Regex α} : [/⊥ ⟨r⟩/] ≃ᵗᵉ [/⊥/] := by
+  simp [TerminatesEquiv, terminates_concat, matchPartial_bot]
+
+theorem terminatesEquiv_concat_bot {r : Regex α} (hr : r.AllTerminates)
+    : [/⟨r⟩ ⊥/] ≃ᵗᵉ [/⊥/] := by
+  simp only [TerminatesEquiv, terminates_concat, terminates_bot, implies_true, exists_prop,
+      and_true, iff_true]
+  exact hr
+
+theorem terminatesEquiv_empty_concat {r : Regex α} : [/ε ⟨r⟩/] ≃ᵗᵉ r := by
+  simp [TerminatesEquiv, terminates_concat, terminates_empty, matchPartial_empty]
+
+theorem terminatesEquiv_concat_empty {r : Regex α} : [/⟨r⟩ ε/] ≃ᵗᵉ r := by
+  simp [TerminatesEquiv, terminates_concat, terminates_empty]
+
+theorem terminatesEquiv_concat_assoc {p q r : Regex α}
+  : [/(⟨p⟩ ⟨q⟩) ⟨r⟩/] ≃ᵗᵉ [/⟨p⟩ (⟨q⟩ ⟨r⟩)/] := by
+  simp only [TerminatesEquiv, terminates_concat, matchPartial_concat, List.mem_flatten,
+    List.mem_pmap, ↓existsAndEq, true_and, forall_exists_index]
+  intro w s cap
+  constructor
+  · rintro ⟨⟨pt, pqt⟩, pqrt⟩; grind
+  · rintro ⟨pt, fn⟩
+    refine ⟨⟨pt, fun mat pm ↦ (fn _ pm).choose⟩, fun mat' mat pm qm ↦ ?_⟩
+    have ⟨qt, qrt⟩ := fn _ pm
+    exact qrt _ qm
+
+theorem terminatesEquiv_or_comm {q r : Regex α}
+    : [/⟨q⟩ | ⟨r⟩/] ≃ᵗᵉ [/⟨r⟩ | ⟨q⟩/] := by
+  simp [TerminatesEquiv, terminates_or, and_comm]
+
+theorem terminatesEquiv_bot_or {r : Regex α} : [/⊥ | ⟨r⟩/] ≃ᵗᵉ r := by
+  simp [TerminatesEquiv, terminates_or, terminates_bot]
+
+theorem terminatesEquiv_or_bot {r : Regex α} : [/⟨r⟩ | ⊥/] ≃ᵗᵉ r := by
+  simp [TerminatesEquiv, terminates_or, terminates_bot]
+
+theorem terminatesEquiv_or_concat {p q r : Regex α}
+    : [/(⟨p⟩ | ⟨q⟩) ⟨r⟩/] ≃ᵗᵉ [/⟨p⟩ ⟨r⟩ | ⟨q⟩ ⟨r⟩/] := by
+  simp only [TerminatesEquiv, terminates_concat, matchPartial_or, List.mem_append, Prod.forall,
+    terminates_or]
+  grind
+
+theorem terminatesEquiv_concat_or {p q r : Regex α}
+    : [/⟨p⟩ (⟨q⟩ | ⟨r⟩)/] ≃ᵗᵉ [/⟨p⟩ ⟨q⟩ | ⟨p⟩ ⟨r⟩/] := by
+  simp only [TerminatesEquiv, terminates_concat, Prod.forall, terminates_or]
+  grind
+
+theorem terminatesEquiv_or_assoc {p q r : Regex α}
+    : [/(⟨p⟩ | ⟨q⟩) | ⟨r⟩/] ≃ᵗᵉ [/⟨p⟩ | (⟨q⟩ | ⟨r⟩)/] := by
+  simp only [TerminatesEquiv, terminates_or]; grind
+
+theorem terminatesEquiv_star_greedy_lazy {r : Regex α} : [/⟨r⟩*/] ≃ᵗᵉ [/⟨r⟩*?/] := by
+  simp only [TerminatesEquiv]
+  intro w s cap
+  induction s using Pos.strongRecEnd generalizing cap with | ind s ind =>
+    rw [terminates_star, terminates_star]; grind
+
+theorem terminatesEquiv_star_type {t} (u : StarType) {r : Regex α}
+    : [/⟨r⟩*‹t›/] ≃ᵗᵉ [/⟨r⟩*‹u›/] := by
+  cases t <;> cases u <;> try rfl
+  · exact terminatesEquiv_star_greedy_lazy
+  · symm; exact terminatesEquiv_star_greedy_lazy
+
+theorem terminatesEquiv_star_bot {t : StarType} : ([/⊥*‹t›/] : Regex α) ≃ᵗᵉ [//] := by
+  rw [TerminatesEquiv]
+  conv in _ ↔ _ => rw [terminates_star]
+  simp [terminates_bot, terminates_empty, matchPartial_bot]
+
+theorem terminatesEquiv_star_empty {t : StarType} : ([/ε*‹t›/] : Regex α) ≃ᵗᵉ [//] := by
+  rw [TerminatesEquiv]
+  conv in _ ↔ _ => rw [terminates_star]
+  simp [terminates_empty, matchPartial_empty]
+
+/-- Whether two regexes are (weakly) matchPartial-equivalent.
+If two regexes are weakly matchPartial-equivalent, you can replace
+membership predicates of `matchPartial` in one regex with the other. -/
+def MatchPartialEquiv (q r : Regex α) := ∃ teq : q ≃ᵗᵉ r,
+  ∀ w s cap term mat,
+    mat ∈ q.matchPartial w s cap term ↔
+    mat ∈ r.matchPartial w s cap ((teq w s cap).mp term)
+
+@[inherit_doc]
+scoped notation:25 q:25 " ≃ʷᵖ " r:26 => MatchPartialEquiv q r
+
+namespace MatchPartialEquiv
+
+theorem terminatesEquiv (heq : q ≃ʷᵖ r) : q ≃ᵗᵉ r := heq.1
+
+@[refl] theorem refl (r : Regex α) : r ≃ʷᵖ r := by simp [MatchPartialEquiv, TerminatesEquiv]
+
+@[symm] theorem symm {q r : Regex α} (qr : q ≃ʷᵖ r) : r ≃ʷᵖ q := by
+  refine ⟨qr.1.symm, ?_⟩; simp [qr.2]
+
+@[trans] theorem trans {p q r : Regex α} (pq : p ≃ʷᵖ q) (qr : q ≃ʷᵖ r)
+    : p ≃ʷᵖ r := by
+  refine ⟨pq.1.trans qr.1, ?_⟩; simp [pq.2, qr.2]
+
+end MatchPartialEquiv
+
+theorem matchPartialEquiv_bot_concat {r : Regex α} : [/⊥ ⟨r⟩/] ≃ʷᵖ [/⊥/] := by
+  refine ⟨terminatesEquiv_bot_concat, ?_⟩
+  simp [matchPartial_concat, matchPartial_bot]
+
+theorem matchPartialEquiv_concat_bot {r : Regex α} (hr : r.AllTerminates)
+    : [/⟨r⟩ ⊥/] ≃ʷᵖ [/⊥/] := by
+  refine ⟨terminatesEquiv_concat_bot hr, ?_⟩
+  simp [matchPartial_concat, matchPartial_bot]
+
+theorem matchPartialEquiv_empty_concat {r : Regex α} : [/ε ⟨r⟩/] ≃ʷᵖ r := by
+  refine ⟨terminatesEquiv_empty_concat, ?_⟩
+  simp [matchPartial_concat, matchPartial_empty]
+
+theorem matchPartialEquiv_concat_empty {r : Regex α} : [/⟨r⟩ ε/] ≃ʷᵖ r := by
+  refine ⟨terminatesEquiv_concat_empty, ?_⟩
+  simp [matchPartial_concat, matchPartial_empty]
+
+theorem matchPartialEquiv_concat_assoc {p q r : Regex α}
+    : [/(⟨p⟩ ⟨q⟩) ⟨r⟩/] ≃ʷᵖ [/⟨p⟩ (⟨q⟩ ⟨r⟩)/] := by
+  refine ⟨terminatesEquiv_concat_assoc, ?_⟩
+  simp only [mem_matchPartial_concat]
+  intro w s cap term mat
+  constructor
+  · rintro ⟨mip, ⟨miq, pm, qm⟩, rm⟩; grind
+  · rintro ⟨mip, pm, miq, qm, rm⟩
+    exact ⟨_, ⟨_, pm, qm⟩, rm⟩
+
+theorem matchPartialEquiv_or_comm {q r : Regex α}
+    : [/⟨q⟩ | ⟨r⟩/] ≃ʷᵖ [/⟨r⟩ | ⟨q⟩/] := by
+  refine ⟨terminatesEquiv_or_comm, ?_⟩
+  simp [mem_matchPartial_or, or_comm]
+
+theorem matchPartialEquiv_bot_or {r : Regex α} : [/⊥ | ⟨r⟩/] ≃ʷᵖ r := by
+  refine ⟨terminatesEquiv_bot_or, ?_⟩
+  simp [matchPartial_or, matchPartial_bot]
+
+theorem matchPartialEquiv_or_bot {r : Regex α} : [/⟨r⟩ | ⊥/] ≃ʷᵖ r :=
+  matchPartialEquiv_or_comm.trans matchPartialEquiv_bot_or
+
+theorem matchPartialEquiv_or_concat {p q r : Regex α}
+    : [/(⟨p⟩ | ⟨q⟩) ⟨r⟩/] ≃ʷᵖ [/⟨p⟩ ⟨r⟩ | ⟨q⟩ ⟨r⟩/] := by
+  refine ⟨terminatesEquiv_or_concat, ?_⟩
+  simp [mem_matchPartial_or, mem_matchPartial_concat]
+  grind
+
+theorem matchPartialEquiv_concat_or {p q r : Regex α}
+    : [/⟨p⟩ (⟨q⟩ | ⟨r⟩)/] ≃ʷᵖ [/⟨p⟩ ⟨q⟩ | ⟨p⟩ ⟨r⟩/] := by
+  refine ⟨terminatesEquiv_concat_or, ?_⟩
+  simp [mem_matchPartial_or, mem_matchPartial_concat]
+  grind
+
+theorem matchPartialEquiv_or_assoc {p q r : Regex α}
+    : [/(⟨p⟩ | ⟨q⟩) | ⟨r⟩/] ≃ʷᵖ [/⟨p⟩ | (⟨q⟩ | ⟨r⟩)/] := by
+  refine ⟨terminatesEquiv_or_assoc, ?_⟩; simp [mem_matchPartial_or]; grind
+
+theorem matchPartialEquiv_star_greedy_lazy {r : Regex α} : [/⟨r⟩*/] ≃ʷᵖ [/⟨r⟩*?/] := by
+  refine ⟨terminatesEquiv_star_greedy_lazy, ?_⟩
+  intro w s cap term mat
+  induction s using Pos.strongRecEnd generalizing cap mat with | ind s ind =>
+    rw [mem_matchPartial_star, mem_matchPartial_star]; grind
+
+theorem matchPartialEquiv_star_type {t} (u : StarType) {r : Regex α}
+    : [/⟨r⟩*‹t›/] ≃ʷᵖ [/⟨r⟩*‹u›/] := by
+  cases t <;> cases u <;> try rfl
+  · exact matchPartialEquiv_star_greedy_lazy
+  · symm; exact matchPartialEquiv_star_greedy_lazy
+
+theorem matchPartialEquiv_star_bot {t : StarType} : ([/⊥*‹t›/] : Regex α) ≃ʷᵖ [//] := by
+  refine ⟨terminatesEquiv_star_bot, ?_⟩
+  conv in _ ↔ _ => rw [mem_matchPartial_star]
+  simp [mem_matchPartial_bot, mem_matchPartial_empty]
+
+theorem matchPartialEquiv_star_empty {t : StarType} : ([/ε*‹t›/] : Regex α) ≃ʷᵖ [//] := by
+  refine ⟨terminatesEquiv_star_empty, ?_⟩
+  conv in _ ↔ _ => rw [mem_matchPartial_star]
+  simp [mem_matchPartial_empty]
+
+/-- Whether two regexes have the same language
+If two regexes have the same language, you can replace
+`isMatch`/`language` of one regex with the other. -/
+def LanguageEquiv (q r : Regex α) := ∃ teq : q ≃ᵗᵉ r,
+  ∀ w term, q.IsMatch w term ↔ r.IsMatch w ((teq w 0 0).mp term)
+
+@[inherit_doc]
+scoped notation:25 q:25 " ≃ˡᵃ " r:26 => LanguageEquiv q r
+
+namespace LanguageEquiv
+
+theorem terminatesEquiv (heq : q ≃ˡᵃ r) : q ≃ᵗᵉ r := heq.1
+
+@[refl] theorem refl (r : Regex α) : r ≃ˡᵃ r := by simp [LanguageEquiv, TerminatesEquiv]
+
+@[symm] theorem symm {q r : Regex α} (qr : q ≃ˡᵃ r) : r ≃ˡᵃ q := by
+  refine ⟨qr.1.symm, ?_⟩; simp [qr.2]
+
+@[trans] theorem trans {p q r : Regex α} (pq : p ≃ˡᵃ q) (qr : q ≃ˡᵃ r)
+    : p ≃ˡᵃ r := by
+  refine ⟨pq.1.trans qr.1, ?_⟩; simp [pq.2, qr.2]
+
+theorem language (heq : q ≃ˡᵃ r) (term : ∀ w, q.Terminates w 0 0)
+    : q.language term = r.language fun w ↦ (heq.1 w 0 0).mp (term w) := by
+  ext w
+  simp only [Regex.language]
+  exact heq.2 w (term w)
+
+end LanguageEquiv
+
+theorem MatchPartialEquiv.languageEquiv (heq : q ≃ʷᵖ r) : q ≃ˡᵃ r := by
+  have ⟨teq, heq⟩ := heq
+  use teq
+  simp only [IsMatch, match'_def, ne_eq, List.filter_eq_nil_iff, decide_eq_true_eq,
+    not_forall, Decidable.not_not]
+  grind
+
+
+theorem languageEquiv_bot_concat {r : Regex α} : [/⊥ ⟨r⟩/] ≃ˡᵃ [/⊥/] :=
+  matchPartialEquiv_bot_concat.languageEquiv
+
+theorem languageEquiv_concat_bot {r : Regex α} (hr : r.AllTerminates)
+    : [/⟨r⟩ ⊥/] ≃ˡᵃ [/⊥/] :=
+  (matchPartialEquiv_concat_bot hr).languageEquiv
+
+theorem languageEquiv_empty_concat {r : Regex α} : [/ε ⟨r⟩/] ≃ˡᵃ r :=
+  matchPartialEquiv_empty_concat.languageEquiv
+
+theorem languageEquiv_concat_empty {r : Regex α} : [/⟨r⟩ ε/] ≃ˡᵃ r :=
+  matchPartialEquiv_concat_empty.languageEquiv
+
+theorem languageEquiv_concat_assoc {p q r : Regex α}
+    : [/(⟨p⟩ ⟨q⟩) ⟨r⟩/] ≃ˡᵃ [/⟨p⟩ (⟨q⟩ ⟨r⟩)/] :=
+  matchPartialEquiv_concat_assoc.languageEquiv
+
+theorem languageEquiv_or_comm {q r : Regex α}
+    : [/⟨q⟩ | ⟨r⟩/] ≃ˡᵃ [/⟨r⟩ | ⟨q⟩/] :=
+  matchPartialEquiv_or_comm.languageEquiv
+
+theorem languageEquiv_bot_or {r : Regex α} : [/⊥ | ⟨r⟩/] ≃ˡᵃ r :=
+  matchPartialEquiv_bot_or.languageEquiv
+
+theorem languageEquiv_or_bot {r : Regex α} : [/⟨r⟩ | ⊥/] ≃ˡᵃ r :=
+  matchPartialEquiv_or_bot.languageEquiv
+
+theorem languageEquiv_or_concat {p q r : Regex α}
+    : [/(⟨p⟩ | ⟨q⟩) ⟨r⟩/] ≃ˡᵃ [/⟨p⟩ ⟨r⟩ | ⟨q⟩ ⟨r⟩/] :=
+  matchPartialEquiv_or_concat.languageEquiv
+
+theorem languageEquiv_concat_or {p q r : Regex α}
+    : [/⟨p⟩ (⟨q⟩ | ⟨r⟩)/] ≃ˡᵃ [/⟨p⟩ ⟨q⟩ | ⟨p⟩ ⟨r⟩/] :=
+  matchPartialEquiv_concat_or.languageEquiv
+
+theorem languageEquiv_or_assoc {p q r : Regex α}
+    : [/(⟨p⟩ | ⟨q⟩) | ⟨r⟩/] ≃ˡᵃ [/⟨p⟩ | (⟨q⟩ | ⟨r⟩)/] :=
+  matchPartialEquiv_or_assoc.languageEquiv
+
+theorem languageEquiv_star_greedy_lazy {r : Regex α} : [/⟨r⟩*/] ≃ˡᵃ [/⟨r⟩*?/] :=
+  matchPartialEquiv_star_greedy_lazy.languageEquiv
+
+theorem languageEquiv_star_type {t} (u : StarType) {r : Regex α}
+    : [/⟨r⟩*‹t›/] ≃ˡᵃ [/⟨r⟩*‹u›/] :=
+  (matchPartialEquiv_star_type u).languageEquiv
+
+theorem languageEquiv_star_bot {t : StarType} : ([/⊥*‹t›/] : Regex α) ≃ˡᵃ [//] :=
+  matchPartialEquiv_star_bot.languageEquiv
+
+theorem languageEquiv_star_empty {t : StarType} : ([/ε*‹t›/] : Regex α) ≃ˡᵃ [//] :=
+  matchPartialEquiv_star_empty.languageEquiv
+
+/-- Whether two regexes are strongly matchPartial-equivalent.
+If two regexes are strongly matchPartial-equivalent, you can replace
+*a sub-regex with the other regex* in
+membership predicate of `matchPartial` -/
+def MatchPartialStrongEquiv (q r : Regex α) := ∃ teq : q ≃ᵗᵉ r,
+  ∀ w s cap term,
+    (q.matchPartial w s cap term).reverse.dedup.reverse =
+    (r.matchPartial w s cap ((teq w s cap).mp term)).reverse.dedup.reverse
+
+@[inherit_doc]
+scoped notation:25 q:25 " ≃ʷᵖ! " r:26 => MatchPartialStrongEquiv q r
+
+theorem MatchPartialStrongEquiv.terminatesEquiv (heq : q ≃ʷᵖ! r) : q ≃ᵗᵉ r := heq.1
+
+theorem MatchPartialStrongEquiv.matchPartialEquiv (heq : q ≃ʷᵖ! r) : q ≃ʷᵖ r := by
+  refine ⟨heq.1, ?_⟩
+  intro w s cap term mat
+  rw [← List.mem_reverse, ← List.mem_dedup, ← List.mem_reverse]
+  rw [heq.2]
+  rw [List.mem_reverse, List.mem_dedup, List.mem_reverse]
+
+--theorem matchPartialStrongEquiv_or_assoc (p q r : Regex α)
+--    : [/(⟨p⟩ | ⟨q⟩) | ⟨r⟩/] ≃ʷᵖ! [/⟨p⟩ | (⟨q⟩ | ⟨r⟩)/] := by
+--  constructor; rotate_left 1
+--  · refl
+
+end Regex
