Regex/Lemmas/Mem.lean
@@ -1,0 +1,95 @@
+import Regex.Termination
+
+/-! Lemmas about `matchPartial` membership -/
+
+namespace Regex
+
+variable {α : Type u} [deq : DecidableEq α] {q r : Regex α} {w : List α}
+  {s : Pos w} {cap : Captures w} {mat : Pos w × Captures w}
+
+theorem mem_matchPartial_bot : ¬mat ∈ [/⊥/].matchPartial w s cap terminates_bot := by
+  simp [matchPartial_bot]
+
+theorem mem_matchPartial_empty
+    : mat ∈ [//].matchPartial w s cap terminates_empty ↔ mat = (s, cap) := by
+  simp [matchPartial_empty]
+
+theorem mem_matchPartial_unit {c : α}
+    : mat ∈ [/c/].matchPartial w s cap terminates_unit ↔
+      ∃ wsc : w[s.val]? = c, mat = (s.succOfIndex wsc, cap) := by
+  simp [matchPartial_unit]
+
+theorem mem_matchPartial_concat {q r : Regex α} (term)
+    : mat ∈ [/⟨q⟩ ⟨r⟩/].matchPartial w s cap term ↔
+      ∃ mid, ∃ mem : mid ∈ q.matchPartial w s cap (terminates_concat.mp term).1,
+        mat ∈ r.matchPartial w mid.1 mid.2 ((terminates_concat.mp term).2 _ mem) := by
+  simp [matchPartial_concat]
+
+theorem mem_matchPartial_or {q r : Regex α} (term)
+    : mat ∈ [/⟨q⟩ | ⟨r⟩/].matchPartial w s cap term ↔
+        mat ∈ q.matchPartial w s cap (terminates_or.mp term).1 ∨
+        mat ∈ r.matchPartial w s cap (terminates_or.mp term).2 := by
+  simp [matchPartial_or]
+
+private theorem mem_dite {t : StarType} {s'} {cap'} {term}
+  : (mat ∈ if _ : s < s' then [/⟨r⟩*‹t›/].matchPartial w s' cap' term else [(s', cap')]) ↔
+    if _ : s < s' then mat ∈ [/⟨r⟩*‹t›/].matchPartial w s' cap' term else mat = (s', cap') := by
+  split <;> simp
+
+theorem mem_matchPartial_star {t : StarType} (term)
+    : mat ∈ [/⟨r⟩*‹t›/].matchPartial w s cap term ↔
+      mat = (s, cap) ∨
+      ∃ mid, ∃ mem : mid ∈ r.matchPartial w s cap (terminates_star.mp term).1,
+        if h : s < mid.1
+          then mat ∈ [/⟨r⟩*‹t›/].matchPartial w mid.1 mid.2
+            ((terminates_star.mp term).2 _ mem h)
+          else mat = mid := by
+  rw [matchPartial_star]
+  simp only [List.cons_append, List.nil_append, Prod.exists]
+  split <;> (
+    simp only [List.mem_append, List.mem_flatten, List.mem_pmap, Prod.exists, ↓existsAndEq,
+      true_and, List.mem_cons, List.not_mem_nil, or_false]
+    try rw [or_comm (b := mat = _)]
+    rw [iff_eq_eq]; congr; ext x;
+    rw [iff_eq_eq]; congr; ext x';
+    rw [iff_eq_eq]; congr; ext x'';
+    rw [iff_eq_eq]
+    split <;> simp
+  )
+
+theorem mem_matchPartial_start
+    : mat ∈ [/⊢/].matchPartial w s cap terminates_start ↔
+      s = 0 ∧ mat = (s, cap) := by
+  simp [matchPartial_start]
+
+theorem mem_matchPartial_end'
+    : mat ∈ [/⊣/].matchPartial w s cap terminates_end' ↔
+      s = w.length ∧ mat = (s, cap) := by
+  simp [matchPartial_end']
+
+theorem mem_matchPartial_capture {n : ℕ} {term}
+    : mat ∈ [/(n ← ⟨r⟩)/].matchPartial w s cap term ↔
+      ∃ mid ∈ r.matchPartial w s cap (terminates_capture.mp term),
+      mat = (mid.1, mid.2.update n [(s, mid.1)]) := by
+  simp [matchPartial_capture, eq_comm (a := mat)]
+
+theorem mem_matchPartial_list {l : List α}
+    : mat ∈ (list l).matchPartial w s cap terminates_list ↔
+      ∃ wsl : w.extract s (s + l.length) = l, mat = (s.addOfIndex wsl rfl, cap) := by
+  simp [matchPartial_list]
+
+theorem mem_matchPartial_backref {d : BackrefDefault} {n : ℕ}
+    : mat ∈ [/\‹d›n/].matchPartial w s cap terminates_backref ↔
+      match (cap n).head? with
+      | none => d = .empty ∧ mat = (s, cap)
+      | some (cs, ct) => ∃ h : w.extract s (s + (ct - cs)) = w.extract cs ct,
+          mat = (s.addOfIndex h (List.length_extract_pos _ _), cap) := by
+  simp only [matchPartial_backref]
+  split <;> split <;> split <;> expose_names
+  all_goals try { simp [*] at * }
+  · simp only [heq, Option.some.injEq, Prod.mk.injEq] at heq_1; simp [← heq_1, h]
+  · simp only [heq, Option.some.injEq, Prod.mk.injEq] at heq_1
+    simp only [← heq_1, h]
+    simp
+
+end Regex
