Regex/Lemmas/Monotone.lean
@@ -1,11 +1,11 @@
-import Regex.Lemmas.Bounds
+import Regex.Lemmas.Equiv
 
 /-! Here we prove monotonicity of regex matches. A regex match does not
 end before it starts. -/
 
 namespace Regex
 variable {α : Type u} [deq : DecidableEq α] {r : Regex α} {w : List α}
-  {s : ℕ} {cap : Captures} {term : r.Terminates w s cap}
+  {s : Pos w} {cap : Captures w} {term : r.Terminates w s cap}
 
 /-- Regexes where matches don't end before they start (all the regexes) -/
 def Monotone (r : Regex α) :=
@@ -14,34 +14,28 @@ def Monotone (r : Regex α) :=
 
 theorem monotone_star {t : StarType} {r : Regex α} (rm : r.Monotone)
     : [/⟨r⟩*‹t›/].Monotone := by
+  rw [Monotone]
+  conv in Terminates _ _ _ _ => rw [terminatesEquiv_star_type .greedy]
+  conv in _ ∈ _ => rw [(matchPartialEquiv_star_type .greedy).2]
   intro w s cap term
-  rcases le_or_gt s w.length with sle | sgt
-  · induction s, sle using decreasingStrongRec generalizing cap with | ind s sle ind =>
-      simp only [matchPartial_star]
-      cases t
-      case greedy | lazy =>
-        simp only [matchPartial_or, matchPartial_filterEmpty, ge_iff_le, eq_iff_iff, iff_true,
-          matchPartial_concat, Bool.false_eq_true, iff_false, not_le, matchPartial_empty,
-          List.append_assoc, List.mem_append, List.mem_filter, decide_eq_true_eq, List.mem_flatten,
-          List.mem_pmap, Prod.exists, ↓existsAndEq, true_and, List.mem_cons, List.not_mem_nil,
-          or_false, Prod.forall, Prod.mk.injEq]
-        intro s' cap' or
-        try rw [or_comm (a := _ ∧ cap' = _), or_assoc] at or
-        rcases or with mem | ⟨s', cap', mem, mem'⟩ | mem
-        · exact rm _ _ _ _ _ mem.1
-        · have bound := endInBounds _ _ sle _ _ _ mem.1
-          exact .trans (rm _ _ _ _ _ mem.1) (ind _ bound mem.2 _ _ _ mem')
-        · simp [mem]
-  · intro mat mem
-    have bound := matchPartial_outOfBounds_eq (le_of_lt sgt) mem
-    simp [bound]
+  induction s using Pos.strongRecEnd generalizing cap with | ind s ind =>
+    conv in _ ∈ _ => rw [matchPartial_star]
+    simp only [List.mem_append, List.mem_flatten, List.mem_pmap, Prod.exists, ↓existsAndEq,
+      true_and, List.mem_cons, List.not_mem_nil, or_false, Prod.forall, Prod.mk.injEq]
+    intro s'' cap'' or
+    rcases or with ⟨s', cap', mem, mem'⟩ | mem
+    · rcases lt_or_eq_of_le (rm _ _ _ _ _ mem) with lt | eq
+      · simp only [lt, ↓reduceDIte] at mem'
+        exact le_of_lt (trans lt (ind _ lt _ ((terminates_star.mp term).2 _ mem lt) _ mem'))
+      · simp [eq] at mem'; simp [eq, mem']
+    · simp [mem]
 
 theorem monotone : r.Monotone := by
   --by_cases! h : s ≤ w.length (by_cases unfolds Monotone and `intro`s variables :( )
   induction r with
   | bot => simp [Monotone, matchPartial_bot]
   | empty => simp [Monotone, matchPartial_empty]
-  | unit _ => simp [Monotone, matchPartial_unit]
+  | unit _ => simp [Monotone, matchPartial_unit, ← Fin.val_fin_le]
   | concat q r qind rind =>
     simp only [Monotone, matchPartial_concat, List.mem_flatten, List.mem_pmap, Prod.exists,
       ↓existsAndEq, true_and, forall_exists_index, Prod.forall]
@@ -54,10 +48,6 @@ theorem monotone : r.Monotone := by
     simp only [Monotone, matchPartial_or, List.mem_append, Prod.forall]
     intro w s cap term s' cap' mem
     exact Or.casesOn mem (fun mem ↦ qind _ _ _ _ _ mem) (fun mem ↦ rind _ _ _ _ _ mem)
-  | filterEmpty e q qind =>
-    simp only [Monotone, matchPartial_filterEmpty, ge_iff_le, eq_iff_iff, Bool.decide_iff_dist,
-      Bool.decide_eq_true, List.mem_filter, beq_iff_eq, and_imp, Prod.forall]
-    exact fun _ _ _ _ _ _ mem _ ↦ qind _ _ _ _ _ mem
   | star t q qind => exact monotone_star qind
   | start => simp [Monotone, matchPartial_start]
   | end' => simp [Monotone, matchPartial_end']
@@ -66,9 +56,9 @@ theorem monotone : r.Monotone := by
       ↓existsAndEq, true_and, forall_exists_index, and_imp, Prod.forall, forall_apply_eq_imp_iff₂]
     exact fun _ _ _ _ _ _ mem ↦ qind _ _ _ _ _ mem
   | backref _ _ =>
-    simp only [Monotone, matchPartial_backref, List.extract_eq_drop_take, List.length_take,
-      List.length_drop, add_tsub_cancel_left, Prod.forall]
+    simp only [Monotone, matchPartial_backref, List.extract_eq_drop_take,
+      add_tsub_cancel_left, Prod.forall]
     intro w s cap term
-    split <;> split <;> simp
+    split <;> split <;> simp [← Fin.val_fin_le]
 
 end Regex
